code/sha3/Hacl.Impl.SHA3.Vec.fsti
@@ -19,8 +19,23 @@ inline_for_extraction noextract
 let state_t (m:m_spec) = lbuffer (element_t m) 25ul
 
 inline_for_extraction noextract
-val absorb_inner_block: #m:m_spec
-  -> rateInBytes:size_t{v rateInBytes > 0 /\ v rateInBytes <= 200}
+let absorb_inner_t (m:m_spec) =
+    rateInBytes:size_t{v rateInBytes > 0 /\ v rateInBytes <= 200}
+  -> b:multibuf (lanes m) 256ul
+  -> s:state_t m ->
+  Stack unit
+  (requires fun h -> live_multi h b /\ live h s /\ disjoint_multi b s /\
+    (forall l. l < lanes m ==> (forall i. (i >= v rateInBytes /\ i < 256) ==>
+      Seq.index (as_seq_multi h b).(|l|) i == u8 0)))
+  (ensures  fun h0 _ h1 -> modifies (loc s) h0 h1 /\
+    as_seq h1 s == V.absorb_inner #m (v rateInBytes) (as_seq_multi h0 b) (as_seq h0 s))
+
+inline_for_extraction noextract
+val absorb_inner: #m:m_spec -> absorb_inner_t m
+
+inline_for_extraction noextract
+let absorb_inner_block_t (m:m_spec) =
+    rateInBytes:size_t{v rateInBytes > 0 /\ v rateInBytes <= 200}
   -> len:size_t
   -> b:multibuf (lanes m) len
   -> i:size_t{v i < v len / v rateInBytes}
@@ -31,8 +46,11 @@ val absorb_inner_block: #m:m_spec
     as_seq h1 s == V.absorb_inner_block #m (v rateInBytes) (v len) (as_seq_multi h0 b) (v i) (as_seq h0 s))
 
 inline_for_extraction noextract
-val absorb_inner_nblocks: #m:m_spec
-  -> rateInBytes:size_t{v rateInBytes > 0 /\ v rateInBytes <= 200}
+val absorb_inner_block: #m:m_spec -> absorb_inner:absorb_inner_t m -> absorb_inner_block_t m
+
+inline_for_extraction noextract
+let absorb_inner_nblocks_t (m:m_spec) =
+    rateInBytes:size_t{v rateInBytes > 0 /\ v rateInBytes <= 200}
   -> len:size_t
   -> b:multibuf (lanes m) len
   -> s:state_t m ->
@@ -42,8 +60,11 @@ val absorb_inner_nblocks: #m:m_spec
     as_seq h1 s == V.absorb_inner_nblocks #m (v rateInBytes) (v len) (as_seq_multi h0 b) (as_seq h0 s))
 
 inline_for_extraction noextract
-val absorb_final: #m:m_spec
-  -> rateInBytes:size_t{v rateInBytes > 0 /\ v rateInBytes <= 200}
+val absorb_inner_nblocks: #m:m_spec -> absorb_inner:absorb_inner_t m -> absorb_inner_nblocks_t m
+
+inline_for_extraction noextract
+let absorb_final_t (m:m_spec) =
+    rateInBytes:size_t{v rateInBytes > 0 /\ v rateInBytes <= 200}
   -> len:size_t
   -> b:multibuf (lanes m) len
   -> delimitedSuffix:byte_t
@@ -55,8 +76,11 @@ val absorb_final: #m:m_spec
       V.absorb_final #m (as_seq h0 s) (v rateInBytes) (v len) (as_seq_multi h0 b) delimitedSuffix)
 
 inline_for_extraction noextract
-val absorb: #m:m_spec
-  -> rateInBytes:size_t{v rateInBytes > 0 /\ v rateInBytes <= 200}
+val absorb_final: #m:m_spec -> absorb_inner:absorb_inner_t m -> absorb_final_t m
+
+inline_for_extraction noextract
+let absorb_t (m:m_spec) =
+    rateInBytes:size_t{v rateInBytes > 0 /\ v rateInBytes <= 200}
   -> len:size_t
   -> b:multibuf (lanes m) len
   -> delimitedSuffix:byte_t
@@ -65,6 +89,9 @@ val absorb: #m:m_spec
   (requires fun h -> live_multi h b /\ live h s /\ disjoint_multi b s)
   (ensures  fun h0 _ h1 -> modifies (loc s) h0 h1 /\
     as_seq h1 s == V.absorb #m (as_seq h0 s) (v rateInBytes) (v len) (as_seq_multi h0 b) delimitedSuffix)
+
+inline_for_extraction noextract
+val absorb: #m:m_spec -> absorb_inner:absorb_inner_t m -> absorb_t m
 
 inline_for_extraction noextract
 val squeeze_nblocks: #m:m_spec
@@ -109,8 +136,8 @@ val squeeze: #m:m_spec
       as_seq_multi h1 b == V.squeeze #m (as_seq h0 s) (v rateInBytes) (v outputByteLen) (as_seq_multi h0 b))
 
 inline_for_extraction noextract
-val keccak: #m:m_spec
-  -> rate:size_t{v rate % 8 == 0 /\ v rate / 8 > 0 /\ v rate <= 1600}
+let keccak_t (m:m_spec) =
+    rate:size_t{v rate % 8 == 0 /\ v rate / 8 > 0 /\ v rate <= 1600}
   -> inputByteLen:size_t
   -> input:multibuf (lanes m) inputByteLen
   -> delimitedSuffix:byte_t
@@ -123,3 +150,6 @@ val keccak: #m:m_spec
       modifies_multi output h0 h1 /\
       as_seq_multi h1 output ==
         V.keccak #m (v rate) (v inputByteLen) (as_seq_multi h0 input) delimitedSuffix (v outputByteLen) (as_seq_multi h0 output))
+
+inline_for_extraction noextract
+val keccak: #m:m_spec -> absorb_inner:absorb_inner_t m -> keccak_t m
